

$$3^2 = 3 \cdot 3 = 27$$

$$x^n = x \cdot x \cdot \dots \cdot x_{n-1} \cdot x$$

CSI Assignment 1

Q2

$$f(n) = \frac{1}{100}n^2 + 100n + 90 \text{ is } O(n^2)$$

$$\frac{1}{100}n^2 \leq C \cdot n^2 \text{ when } C = \frac{1}{100} \text{ for all } n \geq 1$$

$$100n \leq C \cdot n^2 \text{ when } C = 100 \text{ for all } n \geq 100$$

$$90 \leq C \cdot n^2 \text{ when } C = 90 \text{ for all } n \geq 10$$

$$\rightarrow C = \frac{1}{100} + 100 + 90 \quad n_0 = 1$$

$$= \frac{1}{100} + \frac{10000}{100} + \frac{9000}{100}$$

$$= \frac{18001}{100}$$

$$= 180.01$$

True

$$C = \frac{18001}{100}$$

$$n_0 = 1$$

$$\therefore \frac{1}{100}n^2 + 100n + 90 \leq \frac{18001}{100}n^2 \text{ for all } n \geq 1$$

$$\therefore f(n) \in O(n^2) \iff \text{there exists } C, n_0 \text{ such that } f(n) \leq C(n^2) \text{ for all } n \geq n_0$$

b)

$$n \log n + 100 \log n \text{ is } O(\sqrt{n})$$

$$f(n) = n \log n + 100 \log n$$

$$\rightarrow n \log n \geq C \cdot \sqrt{n} \text{ when } C = 1 \quad n \geq 3.585$$

$$n \log n \geq \sqrt{n}$$

$$n \log n \geq \frac{n}{\sqrt{n}}$$

$$n = \frac{n}{\sqrt{n}} \cdot \sqrt{n}$$

$$n \log n \geq \frac{n}{\sqrt{n}}$$

$$n \log n \geq \frac{n}{\sqrt{n}}$$

$$n \log n \geq \sqrt{n}$$

$$\log n \geq \frac{1}{\sqrt{n}}$$

$$\log n \geq \frac{1}{\sqrt{n}}$$

$$n \log n \geq \sqrt{n}$$

$$\log n \geq \frac{1}{\sqrt{n}}$$

$$\log n \geq \frac{1}{\sqrt{n}}$$

$$\sqrt{n} \log n \geq 1$$

$$n \log n \geq \sqrt{n} \quad t = n$$

$$t = n$$

$$\log n \geq \frac{1}{\sqrt{n}}$$

$$\rightarrow t^2 \log t^2 = t$$

$$t = \sqrt{n}$$

$$\sqrt{n} \log n \geq 1$$

$$\rightarrow 2t \log t \geq 1$$

$$t \geq \frac{1}{2}$$

$$n \geq 10^2$$

$$t = 3 = \frac{1}{2}$$

$$t = 3 = \frac{1}{2}$$

$$n \geq 10^2$$

$$1.43 \leq \sqrt{n}$$

$$1.43 \leq \sqrt{n}$$

$$n \geq 10^2$$

Quantity is impossible to solve without advanced mathematics, but can use approximation

b) $\log \log n \geq c \cdot n$ when c is const, for all $n \geq 2$
 $\rightarrow \log \log n \geq \log 2$ const + get exact number
 $\rightarrow \log 2 \geq 1$ we don't have advanced number
 $\rightarrow \log 2 \geq 1$ can use approximation

$n > 0$ \therefore this false due
 $n=1$ $\frac{\log(1)}{1} = 0 \neq 1$ to the inequality
 $n=2$ $\frac{\log(2)}{2} = 0.1505 \neq 1$ no exact solution

c) $(2n+2)^3$ is $\Theta(n^3)$
 Prove: $c_0 g(n) \leq f(n) \leq c_1 g(n)$ for all $n \geq n_0$
 applying to $f(n) = (2n+2)^3$, where $g(n) = n^3$

c_1 part: $(2n+2)^3 \leq c_1 n^3$ $(2n+2)(2n+2)$
 $(2n+2)(2n+2) \leq c_1 n$ $= 4n^2 + 8n + 4$
 $(4n^2 + 12n + 8) \leq c_1 n$ $= 4n^2 + 12n + 8$
 $4n^2 + 12n + 8 \leq c_1 n^3$ $= 4n^2 + 12n + 8$
 $8 + \frac{4}{n} + \frac{12}{n^2} \leq c_1$ $= 8n^3 + 12n^2 + 4n + 8$
 When $c_1 = 110$, $n=1 = 8 + 12 + 4 + 8 = 32$
 For all $n \geq 1$ $= 110$

c_2 : $(2n+2)^3 \geq c_0 \cdot n^3$ let $n \geq 2$
 $8n^3 + 12n^2 + 4n + 8 \geq c_0 n^3$

$c_0 \neq 110$ $110 \geq c_0$
 $n = \frac{110}{2} = 55$ $(1, 55)$
 $x_1 = x_2$ 72 72
 $(2, 216)$
 $2 \cdot$

$$d/dn (2n+2)^3$$

$$= 3(2n+2)^2 \cdot 2$$

$$= 6(2n+2)^2$$

slope at $n=1$

$$6(2(1)+2)^2$$

$$\therefore 6(2n+2)^2 \geq 6n^3 = 6(4)^2$$

$$\text{When } n=1 \text{ for } = 6(12)$$

$$\text{all } n \geq 1$$

$$= 72$$

Proof $8n^3 + 12n^2 + 4n + 18 = 72n^3$

$$2(4n^3 + 2n^2 + 2n + 9) = 36n^3$$

$$4 + \frac{22}{n} + \frac{21}{n^2} + \frac{9}{n^3} = 36$$

True

$$\frac{21}{n} + \frac{21}{n^2} + \frac{9}{n^3} = 32$$

$$\frac{9}{n} (7 + \frac{7}{n} + \frac{1}{n^2}) = 32$$

$$\frac{1}{n} (7 + \frac{7}{n} + \frac{1}{n^2}) = \frac{32}{9}$$

$$\frac{1}{n} \left(\frac{7n^2}{n^2} + \frac{7n}{n^2} + \frac{1}{n^2} \right) = \frac{32}{9}$$

$$\frac{1}{n} \left(\frac{7n^2 + 7n + 1}{n^2} \right) = \frac{32}{9}$$

$$\frac{7n^2 + 7n + 1}{n^3} = \frac{32}{9}$$

$$7n^2 + 7n + 1 = \frac{32}{9}n^3$$

$$n(7n + 7 + \frac{1}{n}) = \frac{32}{9}n^3$$

$$7n + 7 + \frac{1}{n} = \frac{32}{9}n^2$$

$$7 = \frac{32}{9}n^2 - 7n + \frac{1}{n}$$

$$7n = \frac{32}{9}n^3 - 7n^2 + 1$$

$$-8n^3 + 7n^2 + 7n = 3$$

$$n(8n^2 - 7n - 7) = 3$$

$$n(8n^2 - 7n - 7) = 3$$

$$n(8n^2 - 7n - 7) = 3$$

$$n(8n^2 - 7n - 7) = 3$$

$$n(8n^2 - 7n - 7) = 3$$

$$n(8n^2 - 7n - 7) = 3$$

$$n(8n^2 - 7n - 7) = 3$$

$$n(8n^2 - 7n - 7) = 3$$

$$n(8n^2 - 7n - 7) = 3$$

$$n(8n^2 - 7n - 7) = 3$$

$$n(8n^2 - 7n - 7) = 3$$

$$n(8n^2 - 7n - 7) = 3$$

$$n(8n^2 - 7n - 7) = 3$$

$$n(8n^2 - 7n - 7) = 3$$

$$n(8n^2 - 7n - 7) = 3$$

$$n(8n^2 - 7n - 7) = 3$$

$$n(8n^2 - 7n - 7) = 3$$

$$n(8n^2 - 7n - 7) = 3$$

$$n(8n^2 - 7n - 7) = 3$$

$$n(8n^2 - 7n - 7) = 3$$

$$n(8n^2 - 7n - 7) = 3$$

$$n(8n^2 - 7n - 7) = 3$$

$$n(8n^2 - 7n - 7) = 3$$

$$n(8n^2 - 7n - 7) = 3$$

$$n(8n^2 - 7n - 7) = 3$$

$$n(8n^2 - 7n - 7) = 3$$

$$n(8n^2 - 7n - 7) = 3$$

$$n(8n^2 - 7n - 7) = 3$$

$$n(8n^2 - 7n - 7) = 3$$

$$n(8n^2 - 7n - 7) = 3$$

$$n(8n^2 - 7n - 7) = 3$$

$$n(8n^2 - 7n - 7) = 3$$

$$n(8n^2 - 7n - 7) = 3$$

$$n(8n^2 - 7n - 7) = 3$$

$$n(8n^2 - 7n - 7) = 3$$

$$n(8n^2 - 7n - 7) = 3$$

$$n(8n^2 - 7n - 7) = 3$$

$$n(8n^2 - 7n - 7) = 3$$

$$g(n) = 3^n$$

$\Omega(3^n)$ test

$$F(n) \geq 1 \cdot 3^n \quad \therefore K + 3^n \geq 1 \cdot 3^n$$

When $K=1$, for all $n \geq 1$

$F(n) \notin \Omega(g(n)) \Leftrightarrow$ there exists c no such that $F(n) \leq c g(n)$ for all $n \geq n_0$

Θ test

$$\therefore (2^{n+1} + 3^n + n^{100}) \leq (3+K)3^n \text{ for } n \geq 500$$

$(c_0 = 3+K, n_0 = 500)$

$$2^{n+1} + 3^n + n^{100} \geq 3^n \text{ for } n \geq 1 \quad (c_0=1, n_0=1)$$

$\therefore F(n)$ is $\Theta(3^n)$ true.

c) $(1+2+3+\dots+\frac{n}{2})$ is $O(n)$! false,
no c_0 , no exist
 general sequence formula so $f(n) \notin O(n)$

$$(1+2+3+\dots+m) = \frac{n(n+1)}{2} \quad \text{let}$$

$$\text{let } m = \frac{n}{2}$$

$$\rightarrow (1+2+3+\dots+\frac{n}{2}) = \frac{\frac{n}{2}(\frac{n}{2}+1)}{2}$$

$$\therefore \text{it is false} = \frac{1}{2} \cdot \frac{n}{2} \left(\frac{n}{2} + 1 \right)$$

since we take the largest n , in this case n^2 , so $O(n)$

$$= \frac{1}{2} \left(\frac{n^2}{4} + \frac{n}{2} \right) = \frac{n^2}{8} + \frac{n}{4}$$

Questions 2

Q2 a) ~~time~~

time complexity

Step 1 (line 4): 1 (only runs once)
 Step 2 (line 5): n (here n is the length of the array)
 Step 3 (line 6): n
 Step 4 (line 7): 1
 Step 5 (line 8): 1

Worst case time complexity happens if the value getting searched for is at the end of the array.

$\therefore T(n)$ is $O(n)$

b) In this case, the best case scenario is if val that is getting searched for is at the beg start of the array. ~~then~~ The best case scenario, regardless of the length of the array is $O(1)$

The type of inputs are when val is at the start of the array, i.e.

Input: $int[] \text{data} = \{val, 1, 2, 3, \dots, n=4, 11\}$

Step 1 (line 4): 1
 Step 2 (line 5): 1 (only runs once)
 Step 3 (line 6): 1 (only runs once)
 Step 4 (line 7): 1 (only runs once)
 Step 5 (line 8): (won't run for this specific input type)

Question 3:

```
public class ForgetfullStack<E> implements Stack<E>{
```

```
public class Node<E>;
```

```
private E object;
```

```
private Node<E> next;
```

```
private Node<E> prev;
```

```
public Node(){  
    this(null,null,this);  
}
```

```
public Node(E obj, Node<E> n, Node<E> p){  
    object = obj;  
    next = n;  
    prev = p;  
}
```

```
public E getObject() {  
    return object;  
}
```

```
public Node<E> getNext() {  
    return next;  
}
```

```
public Node<E> getPrev() {  
    return prev;  
}
```

```
public void setObject(E newObj) {  
    object = newObj;  
}
```

```
public void setNext(Node<E> newNext) {  
    next = newNext;  
}
```

```
public void setPrev(Node<E> newPrev) {  
    next = newPrev;  
}
```

```
int sz = 0;  
Node<String> head;  
Node<String> dummy;
```

```
head.setPrev(dummy);  
head.setNext(dummy);
```

```
dummy.setPrev(head);  
dummy.setNext(head);
```

```
public int size(){  
    return sz;  
}
```

```
public boolean isEmpty(){  
    return(head.getNext() == dummy);  
}
```

```
public E top(){  
    if(isEmpty()){  
        return null;  
    }  
    else{  
        return head.getNext;  
    }  
}
```

```
public void push(E Object){  
    Node<String> temp = new Node<>(Object, null);  
    if(isEmpty()){  
        head.setNext(temp);  
        dummy.setPrev(temp);  
        temp.setNext(dummy);  
        sz++;  
    }  
    else{  
        Node<String> current = head.getNext;  
        temp.setNext(current);  
        current.setPrev(temp);  
        head.setNext(temp);  
        sz ++;  
    }  
}
```

```
}
```

```
public E pop(){
```

```
if(isEmpty()){
```

```
return null;
```

```
}
```

```
else{
```

```
Node<String> current = head.getNext;
```

```
head.setNext(current.getNext);
```

```
current.getNext.setPrev(head);
```

```
sz --;
```

```
}
```

```
}
```

```
public void forget(int k){
```

```
for(int i = 0; i<k; i++){
```

```
if(sz<=0){return;}
```

```
else{
```

```
Node<String> temp = dummy.getPrev;
```

```
dummy.setPrev(temp.getPrev);
```

```
}
```

```
}
```

```
}
```

```
public static void main(String [] args){  
    ForgetfullStack s = new ForgetfullStack();  
  
    s.push("A");  
    s.push("B");  
    s.push("C");  
    s.push("D");  
    s.push("E");  
    s.push("F");  
    s.pop();  
    s.forget(2);  
}  
}
```

Every method (besides forget) is taken from already confirmed $O(1)$ linked list methods. The reason why 'forget' is $O(1)$ is because it does not traverse the whole stack. All it does is repeat equal to the number given in main. Therefore, since said input is an integer, the time complexity simplifies to $O(1)$.